Start updating the demo and the tutorials

tests/lean/Tutorial/Solutions.lean
@@ -1,6 +1,6 @@
 import Aeneas
 import Tutorial.Tutorial
-open Aeneas.Std Result
+open Aeneas.Std Result WP
 
 set_option maxHeartbeats 1000000
 
@@ -41,7 +41,7 @@ example (a b c d : Prop) (h0 : a → b → c) (h1 : c → d → e)
 
 open CList
 
-@[simp] def CList.toList {α : Type} (x : CList α) : List α :=
+@[simp, grind =] def CList.toList {α : Type} (x : CList α) : List α :=
   match x with
   | CNil => []
   | CCons hd tl => hd :: tl.toList
@@ -49,9 +49,9 @@ open CList
 /-- Theorem about `list_nth_mut1`: verbose version -/
 theorem list_nth_mut1_spec {T: Type} [Inhabited T] (l : CList T) (i : U32)
   (h : i.val < l.toList.length) :
-  ∃ x back, list_nth_mut1 l i = ok (x, back) ∧
-  x = l.toList[i.val]! ∧
-  ∀ x', (back x').toList = l.toList.set i.val x' := by
+  list_nth_mut1 l i ⦃⇓ (x, back) =>
+    x = l.toList[i.val]! ∧
+    ∀ x', (back x').toList = l.toList.set i.val x' ⦄ := by
   unfold list_nth_mut1 list_nth_mut1_loop
   split
   . rename_i hd tl
@@ -89,7 +89,7 @@ theorem list_nth_mut1_spec {T: Type} [Inhabited T] (l : CList T) (i : U32)
         simp only [hiEq]
   . simp_all
 
-/-- Theorem about `list_nth_mut1`: simple version.
+/-- Theorem about `list_nth_mut1`: simpler version.
 
     Remark: a simple way of simplifying the context is simply to
     call `simp_all`. Below, we're trying to be a bit more precise with
@@ -98,9 +98,9 @@ theorem list_nth_mut1_spec {T: Type} [Inhabited T] (l : CList T) (i : U32)
  -/
 theorem list_nth_mut1_spec' {T: Type} [Inhabited T] (l : CList T) (i : U32)
   (h : i.val < l.toList.length) :
-  ∃ x back, list_nth_mut1 l i = ok (x, back) ∧
-  x = l.toList[i.val]! ∧
-  ∀ x', (back x').toList = l.toList.set i.val x' := by
+  list_nth_mut1 l i ⦃⇓ (x, back) =>
+    x = l.toList[i.val]! ∧
+    ∀ x', (back x').toList = l.toList.set i.val x' ⦄ := by
   unfold list_nth_mut1 list_nth_mut1_loop
   split
   . split
@@ -120,13 +120,23 @@ theorem list_nth_mut1_spec' {T: Type} [Inhabited T] (l : CList T) (i : U32)
         simp [*]
   . simp_all
 
+/- Even simpler: `progress*` can do most of the work -/
+theorem list_nth_mut1_spec'' {T: Type} [Inhabited T] (l : CList T) (i : U32)
+  (h : i.val < l.toList.length) :
+  list_nth_mut1 l i ⦃⇓ (x, back) =>
+    x = l.toList[i.val]! ∧
+    ∀ x', (back x').toList = l.toList.set i.val x' ⦄ := by
+  unfold list_nth_mut1 list_nth_mut1_loop
+  progress* <;> try grind
+  simp_all
+
 /-- Theorem about `list_tail_loop`: verbose version -/
 @[progress]
 theorem list_tail_loop_spec {T : Type} (l : CList T) :
-  ∃ back, list_tail_loop l = ok back ∧
-  ∀ tl', (back tl').toList = l.toList ++ tl'.toList := by
+  list_tail_loop l ⦃⇓ back =>
+    ∀ tl', (back tl').toList = l.toList ++ tl'.toList ⦄ := by
   unfold list_tail_loop
-  split
+  cases h: l
   . rename_i hd tl
     simp
     progress as ⟨ back, hBack ⟩
@@ -142,41 +152,42 @@ theorem list_tail_loop_spec {T : Type} (l : CList T) :
 /-- Theorem about `list_tail_loop: simple version -/
 @[progress]
 theorem list_tail_loop_spec' {T : Type} (l : CList T) :
-  ∃ back, list_tail_loop l = ok back ∧
-  ∀ tl', (back tl').toList = l.toList ++ tl'.toList := by
+  list_tail_loop l ⦃⇓ back =>
+    ∀ tl', (back tl').toList = l.toList ++ tl'.toList ⦄ := by
   unfold list_tail_loop
   progress*
 
 @[progress]
 theorem list_tail_spec {T : Type} (l : CList T) :
-  ∃ back, list_tail l = ok (CList.CNil, back) ∧
-  ∀ tl', (back tl').toList = l.toList ++ tl'.toList := by
+  list_tail l ⦃⇓ (tl, back) =>
+    tl = CNil ∧
+    ∀ tl', (back tl').toList = l.toList ++ tl'.toList ⦄ := by
   unfold list_tail
   progress*
 
 /-- Theorem about `append_in_place` -/
 @[progress]
 theorem append_in_place_spec {T : Type} (l0 l1 : CList T) :
-  ∃ l2, append_in_place l0 l1 = ok l2 ∧
-  l2.toList = l0.toList ++ l1.toList := by
+  append_in_place l0 l1 ⦃⇓ l2 =>
+    l2.toList = l0.toList ++ l1.toList ⦄ := by
   unfold append_in_place
   progress as ⟨ tl, back ⟩
-  progress as ⟨ l2 ⟩
+  grind
 
 @[progress]
 theorem reverse_loop_spec {T : Type} (l : CList T) (out : CList T) :
-  ∃ l', reverse_loop l out = ok l' ∧
-  l'.toList = l.toList.reverse ++ out.toList := by
+  reverse_loop l out ⦃⇓ l' =>
+    l'.toList = l.toList.reverse ++ out.toList ⦄ := by
   unfold reverse_loop
-  split
+  cases h: l
   . progress as ⟨ l1, hl1 ⟩
     simp at *
     simp [hl1]
   . simp
 
 theorem reverse_spec {T : Type} (l : CList T) :
-  ∃ l', reverse l = ok l' ∧
-  l'.toList = l.toList.reverse := by
+  reverse l ⦃⇓ l' =>
+    l'.toList = l.toList.reverse ⦄ := by
   unfold reverse
   progress as ⟨ l', hl' ⟩
   simp at hl'
@@ -200,11 +211,10 @@ def toInt (l : List U32) : Int :=
 @[progress]
 theorem zero_loop_spec
   (x : alloc.vec.Vec U32) (i : Usize) (h : i.val ≤ x.length) :
-  ∃ x',
-    zero_loop x i = ok x' ∧
+  zero_loop x i ⦃⇓ x' =>
     x'.length = x.length ∧
     (∀ j, j < i.val → x'[j]! = x[j]!) ∧
-    (∀ j, i.val ≤ j → j < x.length → x'[j]! = 0#u32) := by
+    (∀ j, i.val ≤ j → j < x.length → x'[j]! = 0#u32) ⦄ := by
   unfold zero_loop
   simp
   split
@@ -241,10 +251,9 @@ theorem all_nil_impl_toInt_eq_zero
 
 /-- The theorem about `zero` -/
 theorem zero_spec (x : alloc.vec.Vec U32) :
-  ∃ x',
-    zero x = ok x' ∧
+  zero x ⦃⇓ x' =>
     x'.length = x.length ∧
-    toInt x' = 0 := by
+    toInt x' = 0 ⦄ := by
   unfold zero
   progress as ⟨ x', hLength, hSame, hZero ⟩
   simp_all
@@ -312,9 +321,9 @@ theorem add_no_overflow_loop_spec
   (hLength : x.length = y.length)
   -- No overflow occurs when we add the individual thunks
   (hNoOverflow : ∀ (j : Nat), i.val ≤ j → j < x.length → x[j]!.val + y[j]!.val ≤ U32.max) :
-  ∃ x', add_no_overflow_loop x y i = ok x' ∧
-  x'.length = x.length ∧
-  toInt x' = toInt x + 2 ^ (32 * i.val) * toInt (y.val.drop i.val) := by
+  add_no_overflow_loop x y i ⦃⇓ x' =>
+    x'.length = x.length ∧
+    toInt x' = toInt x + 2 ^ (32 * i.val) * toInt (y.val.drop i.val) ⦄ := by
   unfold add_no_overflow_loop
   simp
   split
@@ -352,9 +361,9 @@ decreasing_by scalar_decr_tac
 theorem add_no_overflow_spec (x : alloc.vec.Vec U32) (y : alloc.vec.Vec U32)
   (hLength : x.length = y.length)
   (hNoOverflow : ∀ (j : Nat), j < x.length → x[j]!.val + y[j]!.val ≤ U32.max) :
-  ∃ x', add_no_overflow x y = ok x' ∧
-  x'.length = y.length ∧
-  toInt x' = toInt x + toInt y := by
+  add_no_overflow x y ⦃⇓ x' =>
+    x'.length = y.length ∧
+    toInt x' = toInt x + toInt y ⦄ := by
   unfold add_no_overflow
   progress as ⟨ x' ⟩ <;>
   simp_all
@@ -366,11 +375,11 @@ theorem add_with_carry_loop_spec
   (hLength : x.length = y.length)
   (hi : i.val ≤ x.length)
   (hCarryLe : c0.val ≤ 1) :
-  ∃ x' c1, add_with_carry_loop x y c0 i = ok (c1, x') ∧
-  x'.length = x.length ∧
-  c1.val ≤ 1 ∧
-  toInt x' + c1.val * 2 ^ (32 * x'.length) =
-    toInt x + 2 ^ (32 * i.val) * toInt (y.val.drop i.val) + c0.val * 2 ^ (32 * i.val) := by
+  add_with_carry_loop x y c0 i ⦃⇓ (c1, x') =>
+    x'.length = x.length ∧
+    c1.val ≤ 1 ∧
+    toInt x' + c1.val * 2 ^ (32 * x'.length) =
+      toInt x + 2 ^ (32 * i.val) * toInt (y.val.drop i.val) + c0.val * 2 ^ (32 * i.val) ⦄ := by
   unfold add_with_carry_loop
   simp
   split
@@ -435,10 +444,10 @@ decreasing_by scalar_decr_tac
 theorem add_with_carry_spec
   (x : alloc.vec.Vec U32) (y : alloc.vec.Vec U32)
   (hLength : x.length = y.length) :
-  ∃ x' c, add_with_carry x y = ok (c, x') ∧
-  x'.length = x.length ∧
-  c.val ≤ 1 ∧
-  toInt x' + c.val * 2 ^ (32 * x'.length) = toInt x + toInt y := by
+  add_with_carry x y ⦃⇓ (c, x') =>
+    x'.length = x.length ∧
+    c.val ≤ 1 ∧
+    toInt x' + c.val * 2 ^ (32 * x'.length) = toInt x + toInt y ⦄ := by
   unfold add_with_carry
   progress as ⟨ c, x' ⟩
   simp_all
